fix bvapp argument order in spec, wip bootloader verification

src/verification/BlockVer/Examples.v
@@ -30,17 +30,16 @@ Import Erasure.notations.
 Module Examples.
   Import Utils.
 
-  Definition asn_ipe_registers {Σ} : Assertion Σ :=
-      ∃ "ipectl", MPUIPC0_reg          ↦ term_var "ipectl"
-    ∗ ∃ "segb1" , MPUIPSEGB1_reg       ↦ term_var "segb1"
-    ∗ ∃ "segb2" , MPUIPSEGB2_reg       ↦ term_var "segb2".
+  Definition asn_ipe_registers_zero {Σ} : Assertion Σ :=
+      MPUIPC0_reg    ↦ term_val ty.wordBits [bv 0]
+    ∗ MPUIPSEGB1_reg ↦ term_val ty.wordBits [bv 0]
+    ∗ MPUIPSEGB2_reg ↦ term_val ty.wordBits [bv 0].
 
   Definition minimal_pre {Σ} (include_ipe : bool) : Assertion Σ :=
       ∃ "lif", LastInstructionFetch ↦ term_var "lif"
     ∗ ∃ "srcg1", SRCG1_reg ↦ term_var "srcg1"
-    ∗ if include_ipe then asn_ipe_registers else ⊤
+    ∗ (* if include_ipe then asn_ipe_registers else *) ⊤
     ∗ asn_mpu_registers.
-
 
   Definition minimal_post {Σ} (include_ipe : bool) : Assertion Σ :=
     minimal_pre include_ipe.
@@ -92,7 +91,7 @@ Module Examples.
   Definition ex_mov_register : BlockVerifierContract :=
     {{
         asn_init_pc (term_val ty.Address [bv 0]) ∗
-        asn_ipe_registers ∗
+        asn_ipe_registers_zero ∗
         R4_reg ↦ term_val ty.wordBits [bv 42] ∗
         ∃ "v", R5_reg ↦ term_var "v"
     }}
@@ -100,7 +99,7 @@ Module Examples.
     [mov_rr R4 R5]
 
     {{
-        asn_ipe_registers ∗
+        asn_ipe_registers_zero ∗
         R4_reg ↦ term_val ty.wordBits [bv 42] ∗
         R5_reg ↦ term_val ty.wordBits [bv 42]
     }}.
@@ -122,134 +121,130 @@ Module Examples.
     Definition asn_byte_zero {Σ} (b : Term Σ ty.byteBits) : Assertion Σ :=
       b = term_val ty.byteBits [bv 0].
 
-    Definition saved_ptr_loc {Σ} : Term Σ _ := term_val ty.Address [bv 0x4242].
+    Definition saved_ptr_loc {Σ} : Term Σ _ := term_val ty.Address [bv 0x4200].
+    Definition saved_ptr {Σ} : Term Σ _ := term_val ty.Address [bv 0x4202].
+    Definition conf_ipectl {Σ} : Term Σ _ := term_val ty.Address [bv 0x00CD].
+    Definition conf_segb1 {Σ} : Term Σ _ := term_val ty.Address [bv 0x6000].
+    Definition conf_segb2 {Σ} : Term Σ _ := term_val ty.Address [bv 0x6100].
+
+    Definition byte_zero {Σ} : Term Σ _ := term_val ty.byteBits [bv 0].
+
     Definition valid_flag {Σ} : Term Σ _ := term_val ty.wordBits [bv 0xAAAA].
     Definition ipe_sig_valid_src {Σ} : Term Σ _ := term_val ty.Address [bv 0xFF88].
     Definition ipe_struct_pointer_src {Σ} : Term Σ _ := term_val ty.Address [bv 0xFF8A].
 
     Definition start_bootcode_start{Σ} : Term Σ _ := term_val ty.wordBits [bv 0].
-    Definition transfer_if_valid_struct_start {Σ} : Term Σ _ := term_val ty.wordBits [bv 0x6].
-    Definition check_struct_start {Σ} : Term Σ _ := term_val ty.wordBits [bv 0x14].
-    Definition evaluate_struct_start {Σ} : Term Σ _ := term_val ty.wordBits [bv 0x24].
-    Definition mass_erase_start {Σ} : Term Σ _ := term_val ty.wordBits [bv 0x38].
-    Definition end_addr {Σ} : Term Σ _ := term_val ty.wordBits [bv 0x48].
+    Definition transfer_if_valid_struct_start {Σ} : Term Σ _ := term_val ty.wordBits [bv 0x4].
+    Definition check_struct_start {Σ} : Term Σ _ := term_val ty.wordBits [bv 0xC].
+    Definition evaluate_struct_start {Σ} : Term Σ _ := term_val ty.wordBits [bv 0x20].
+    Definition mass_erase_start {Σ} : Term Σ _ := term_val ty.wordBits [bv 0x2A].
+    Definition end_addr {Σ} : Term Σ _ := term_val ty.wordBits [bv 0x38].
 
     Definition asn_flag_valid {Σ} : Assertion Σ :=
       asn_ptsto_word ipe_sig_valid_src (low valid_flag) (high valid_flag).
 
+    Definition asn_conf {Σ} : Assertion Σ :=
+        saved_ptr      m↦ low  conf_ipectl
+      ∗ saved_ptr +' 1 m↦ high conf_ipectl
+      ∗ saved_ptr +' 2 m↦ low  conf_segb2
+      ∗ saved_ptr +' 3 m↦ high conf_segb2
+      ∗ saved_ptr +' 4 m↦ low  conf_segb1
+      ∗ saved_ptr +' 5 m↦ high conf_segb1.
+
     Definition contract_start_bootcode : BlockVerifierContract :=
       {{
             asn_init_pc start_bootcode_start
+          ∗ asn_ipe_registers_zero
 
           ∗ R10_reg ↦ saved_ptr_loc
-          ∗ asn_ptsto_word saved_ptr_loc (term_var "ptr_l") (term_var "ptr_h")
+          ∗ (asn_ptsto_word saved_ptr_loc byte_zero byte_zero
+             ∨ asn_ptsto_word saved_ptr_loc (low saved_ptr) (high saved_ptr))
       }}
         [ tst_m R10
-        ; jnz [bv 5] (* check_struct *) ]
+        ; jnz [bv 4] (* check_struct *)]
       {{
             R10_reg ↦ saved_ptr_loc
-          ∗ asn_ptsto_word saved_ptr_loc (term_var "ptr_l") (term_var "ptr_h")
-
-          ∗ (( (*asn_byte_zero (term_var "ptr_l")
-             ∗ asn_byte_zero (term_var "ptr_h")
-             ∗ *)asn_fin_pc transfer_if_valid_struct_start)
-            ∨ asn_fin_pc check_struct_start)
-      }}
-        with ["ptr_l" :: ty.byteBits; "ptr_h" :: ty.byteBits].
+          ∗ asn_ipe_registers_zero
+          ∗ ( asn_ptsto_word saved_ptr_loc byte_zero byte_zero
+                ∗ asn_fin_pc transfer_if_valid_struct_start
+              ∨ asn_ptsto_word saved_ptr_loc (low saved_ptr) (high saved_ptr)
+                ∗ asn_fin_pc check_struct_start)
+      }}.
 
     Definition contract_transfer_if_valid_struct : BlockVerifierContract :=
       {{
             asn_init_pc transfer_if_valid_struct_start
 
+          ∗ asn_ipe_registers_zero
           ∗ R10_reg ↦ saved_ptr_loc
           ∗ R11_reg ↦ valid_flag
           ∗ R12_reg ↦ ipe_sig_valid_src
           ∗ R13_reg ↦ ipe_struct_pointer_src
+
           ∗ asn_flag_valid
-          ∗ asn_ptsto_word ipe_struct_pointer_src
-              (term_var "struct_ptr_l") (term_var "struct_ptr_h")
-          ∗ ∃ "l", ∃ "h", asn_ptsto_word saved_ptr_loc (term_var "l") (term_var "h")
+          ∗ asn_ptsto_word ipe_struct_pointer_src (low saved_ptr) (high saved_ptr)
+          ∗ asn_ptsto_word saved_ptr_loc byte_zero byte_zero
       }}
         [ cmp_rm R11 R12
-        ; jnz [bv 29]
+        ; jnz [bv 0x34] (* TODO end *)
         ; mov_mm R13 R10 ]
       {{
-            R10_reg ↦ saved_ptr_loc
+            asn_fin_pc check_struct_start
+
+          ∗ asn_ipe_registers_zero
+          ∗ R10_reg ↦ saved_ptr_loc
           ∗ R11_reg ↦ valid_flag
           ∗ R12_reg ↦ ipe_sig_valid_src
           ∗ R13_reg ↦ ipe_struct_pointer_src
-          ∗ asn_flag_valid
-          ∗ asn_ptsto_word ipe_struct_pointer_src
-              (term_var "struct_ptr_l") (term_var "struct_ptr_h")
 
-          ∗ asn_fin_pc check_struct_start
-          ∗ asn_ptsto_word saved_ptr_loc (term_var "struct_ptr_l") (term_var "struct_ptr_h")
-      }}
-        with ["struct_ptr_l" :: ty.byteBits; "struct_ptr_h" :: ty.byteBits].
+          ∗ asn_flag_valid
+          ∗ asn_ptsto_word ipe_struct_pointer_src (low saved_ptr) (high saved_ptr)
+          ∗ asn_ptsto_word saved_ptr_loc (low saved_ptr) (high saved_ptr)
+      }}.
 
     Definition contract_evaluate_struct : BlockVerifierContract :=
       {{
-           asn_init_pc evaluate_struct_start
-         ∗ asn_ipe_registers
+           (* asn_init_pc evaluate_struct_start *)
+⊤
+         ∗ asn_ipe_registers_zero
+         ∗ R6_reg ↦ saved_ptr +' 6
+         ∗ R7_reg ↦ MPUIPC0_addr
+         ∗ R8_reg ↦ MPUIPSEGB2_addr
+         ∗ R9_reg ↦ MPUIPSEGB1_addr
 
-         ∗ R6_reg ↦ term_val ty.Address [bv 0x1000]
-         ∗ asn_ptsto_word (term_val ty.Address [bv 0x1000]) (term_val ty.byteBits [bv 0]) (term_val ty.byteBits [bv 0])
-
-         (* ∗ R7_reg ↦ MPUIPC0_addr *)
-         (* ∗ R8_reg ↦ MPUIPSEGB2_addr *)
-         (* ∗ R9_reg ↦ MPUIPSEGB1_addr *)
-
-         (* ∗ R6_reg ↦ term_var "struct_ptr" +' 6 *)
-
-         (* ∗ term_var "struct_ptr" = term_val ty.wordBits [bv 0x1000] *)
-
-         (* (* struct doesn't overlap MPU register file *) *)
-         (* (*    needs more preconditions to exclude overflow of struct_ptr + 6 *) *)
-         (* (* ∗ (term_unsigned (term_var "struct_ptr" +' 6) < (term_val ty.int 0x05A0%Z) *) *)
-         (* (*    ∨ term_val ty.int 0x05B0%Z <= term_unsigned (term_var "struct_ptr")) *) *)
-
-         (* ∗ asn_ptsto_word (term_var "struct_ptr" +' 4) *)
-         (*     (low (term_var "segb1")) (high (term_var "segb1")) *)
-         (* ∗ asn_ptsto_word (term_var "struct_ptr" +' 2) *)
-         (*     (low (term_var "segb2")) (high (term_var "segb2")) *)
-         (* ∗ asn_ptsto_word (term_var "struct_ptr") *)
-         (*     (low (term_var "ipectl")) (high (term_var "ipectl")) *)
+         ∗ asn_ptsto_word (saved_ptr +' 4) (low conf_segb1) (high conf_segb1)
+         (* ∗ asn_ptsto_word (saved_ptr +' 2) (low conf_segb2) (high conf_segb2) *)
+         (* ∗ asn_ptsto_word saved_ptr (low conf_ipectl) (high conf_ipectl) *)
       }}
-        [ mov_rm R6 R6          (* fix offsets *)
+        [ mov_ir R6 (bv.of_Z (-2)%Z) R9
           (* mov_im R6 (bv.of_Z (-2)%Z) R9 *)
         (* ; mov_im R6 (bv.of_Z (-4)%Z) R8 *)
         (* ; mov_im R6 (bv.of_Z (-6)%Z) R7 *)
-        (* ; jump JMP [bv (* 0x08 *) 0x10] *) (* end *)]
-      {{ ⊥
-         (*   (* asn_fin_pc end_addr *) *)
-         (*   PC_reg         ↦ end_addr *)
-         (* ∗ MPUIPC0_reg    ↦ term_var "ipectl" *)
-         (* ∗ MPUIPSEGB1_reg ↦ term_var "segb1" *)
-         (* ∗ MPUIPSEGB2_reg ↦ term_var "segb2" *)
+        (* ; jump JMP [bv 0x7] *) (* end *) ]
+      {{ ⊤
+         (*   asn_fin_pc end_addr *)
 
-         (* ∗ R6_reg ↦ term_var "struct_ptr" +' 6 *)
+           (* MPUIPC0_reg    ↦ conf_ipectl *)
+         (* ∗ MPUIPSEGB1_reg ↦ conf_segb1 *)
+         (* ∗ MPUIPSEGB2_reg ↦ conf_segb2 *)
+
+         (* ∗ R6_reg ↦ saved_ptr +' 6 *)
          (* ∗ R7_reg ↦ MPUIPC0_addr *)
          (* ∗ R8_reg ↦ MPUIPSEGB2_addr *)
          (* ∗ R9_reg ↦ MPUIPSEGB1_addr *)
-      }}
-        with ["ipectl" :: ty.wordBits; "segb1" :: ty.wordBits; "segb2" :: ty.wordBits; "struct_ptr" :: ty.Address].
+
+         (* ∗ asn_ptsto_word (saved_ptr +' 4) (low conf_segb1) (high conf_segb1) *)
+         (* ∗ asn_ptsto_word (saved_ptr +' 2) (low conf_segb2) (high conf_segb2) *)
+         (* ∗ asn_ptsto_word saved_ptr (low conf_ipectl) (high conf_ipectl) *)
+      }}.
 
     Lemma valid_start_bootcode : ValidBlockVerifierContract contract_start_bootcode.
-    Proof. vm_compute. Set Printing Depth 200. Unset Printing 
-           (* 0xe/0x4 = 0x14 *)
-           symbolic_simpl.
-           repeat split; try lia.
-           intuition.
-           auto 10 with *.
-           repeat split.
+    Proof. now symbolic_simpl. Qed.
 
-           vm_compute. Set Printing Depth 200.
-    Qed.
+    Lemma valid_transfer_if_valid_struct : ValidBlockVerifierContract contract_transfer_if_valid_struct.
+    Proof. symbolic_simpl. intros. rewrite H. intuition. Qed.
 
-    (* Lemma valid_transfer_if_valid_struct : ValidBlockVerifierContract contract_transfer_if_valid_struct. *)
-    (* Proof. vm_compute.  *)
-
-    Lemma valid_evaluate_struct : ValidBlockVerifierContractWithExplicitIPE contract_evaluate_struct.
+    Lemma valid_evaluate_struct : ValidBlockVerifierContract contract_evaluate_struct.
     Proof.
       symbolic_simpl.
       repeat right.
@@ -257,278 +252,5 @@ Module Examples.
       intuition; discriminate.
     Qed.
 
-    (* TODO is check_byte_access's contract good enough? *)
-
   End Bootcode.
 End Examples.
-
-(*
-{|
-debug_consume_chunk_pathcondition :=
-[formula_relop
-bop.eq
-(term_var
-"struct_ptr" +' 0x4)
-(term_binop
-bop.bvand
-(term_var
-"struct_ptr" +' 0x4)
-(term_val
-ty.Address
-[bv 0xfffe]));
-formula_relop
-bop.eq
-(term_var
-"struct_ptr" +' 0x2)
-(term_binop
-bop.bvand
-(term_var
-"struct_ptr" +' 0x2)
-(term_val
-ty.Address
-[bv 0xfffe]));
-formula_relop
-bop.eq
-(term_var
-"struct_ptr")
-(term_binop
-bop.bvand
-(term_var
-"struct_ptr")
-(term_val
-ty.Address
-[bv 0xfffe]));
-formula_relop
-bop.eq
-(term_var "bh.1" @
-term_var "bl.1")
-(term_val
-ty.Address
-[bv 0xfffe]);
-formula_relop
-bop.eq
-(term_binop
-bop.bvadd
-(term_var
-"struct_ptr")
-(term_var "bh.1" @
-term_var "bl.1") +'
-0x6)
-(term_binop
-bop.bvand
-(term_binop
-bop.bvadd
-(term_var
-"struct_ptr")
-(term_var "bh.1" @
-term_var "bl.1") +'
-0x6)
-(term_val
-ty.Address
-[bv 0xfffe]));
-formula_relop
-bop.eq
-(term_binop
-bop.bvadd
-(term_var
-"struct_ptr")
-(term_var "bh.1" @
-term_var "bl.1") +'
-0x6)
-(term_var
-"struct_ptr" +' 0x4);
-formula_relop
-bop.eq
-(term_binop
-bop.bvor
-(term_binop
-bop.bvadd
-(term_var
-"struct_ptr")
-(term_var "bh.1" @
-term_var "bl.1") +'
-0x6)
-(term_val
-ty.Address [bv 0x1]))
-(term_binop
-bop.bvor
-(term_var
-"struct_ptr" +' 0x4)
-(term_val
-ty.Address [bv 0x1]));
-formula_relop
-bop.le
-(term_val ty.int
-1456%Z)
-(term_unsigned
-(term_binop
-bop.bvadd
-(term_var
-"struct_ptr")
-(term_var "bh.1" @
-term_var "bl.1") +'
-0x6));
-formula_relop
-bop.le
-(term_val ty.int
-1456%Z)
-(term_unsigned
-(term_binop
-bop.bvor
-(term_binop
-bop.bvadd
-(term_var
-"struct_ptr")
-(term_var "bh.1" @
-term_var "bl.1") +'
-0x6)
-(term_val
-ty.Address [bv 0x1])))];
-debug_consume_chunk_heap :=
-[chunk_ptsreg
-R9_reg
-(term_vector_subrange
-0 8
-(term_var "segb1") @
-term_vector_subrange
-8 8
-(term_var "segb1"));
-chunk_ptsreg
-LastInstructionFetch
-(term_val
-(ty.union Uwordbyte)
-(Word [bv 0x0]));
-chunk_ptsreg
-MPUIPSEGB2_reg
-(term_var "segb2.2");
-chunk_ptsreg
-MPUIPSEGB1_reg
-(term_var "segb1.2");
-chunk_ptsreg
-MPUIPC0_reg
-(term_var
-"ipectl.2");
-chunk_user ptstomem
-[term_binop
-bop.bvor
-(term_binop
-bop.bvadd
-(term_var
-"struct_ptr")
-(term_var "bh.1" @
-term_var "bl.1") +'
-0x6)
-(term_val
-ty.Address [bv 0x1]);
-term_vector_subrange
-0 8
-(term_var "segb1")];
-chunk_user ptstomem
-[term_binop
-bop.bvadd
-(term_var
-"struct_ptr")
-(term_var "bh.1" @
-term_var "bl.1") +'
-0x6;
-term_vector_subrange
-8 8
-(term_var "segb1")];
-chunk_user
-ptstoinstr
-[term_val
-ty.Address
-[bv 0x26];
-term_union
-Uinstr_or_data Kd
-(term_var "bh.1" @
-term_var "bl.1")];
-chunk_ptsreg R6_reg
-(term_var
-"struct_ptr" +' 0x6);
-chunk_user
-ptstoinstr
-[term_val
-ty.Address
-[bv 0x24];
-term_union
-Uinstr_or_data Kd
-(term_var "bh" @
-term_var "bl")];
-chunk_user
-encodes_instr
-[term_var "bh" @
-term_var "bl";
-term_val
-(ty.union Uast)
-(DOUBLEOP MOV
-WORD_INSTRUCTION R6
-INDEXED_MODE R9
-REGISTER_MODE)];
-chunk_user ptstomem
-[term_binop
-bop.bvor
-(term_var
-"struct_ptr")
-(term_val
-ty.Address [bv 0x1]);
-term_vector_subrange
-0 8
-(term_var "ipectl")];
-chunk_user ptstomem
-[term_var
-"struct_ptr";
-term_vector_subrange
-8 8
-(term_var "ipectl")];
-chunk_user ptstomem
-[term_binop
-bop.bvor
-(term_var
-"struct_ptr" +' 0x2)
-(term_val
-ty.Address [bv 0x1]);
-term_vector_subrange
-0 8
-(term_var "segb2")];
-chunk_user ptstomem
-[term_var
-"struct_ptr" +' 0x2;
-term_vector_subrange
-8 8
-(term_var "segb2")];
-chunk_ptsreg R8_reg
-(term_val
-ty.Address
-[bv 0x5ac]);
-chunk_ptsreg R7_reg
-(term_val
-ty.Address
-[bv 0x5aa]);
-chunk_ptsreg
-MPUIPSEGB2_reg
-(term_var "segb2.1");
-chunk_ptsreg
-MPUIPSEGB1_reg
-(term_var "segb1.1");
-chunk_ptsreg
-MPUIPC0_reg
-(term_var
-"ipectl.1")]%list;
-debug_consume_chunk_chunk :=
-chunk_user
-ptstoinstr
-[term_val
-ty.Address
-[bv 0x24];
-term_val
-(ty.union
-Uinstr_or_data)
-(I
-(DOUBLEOP MOV
-WORD_INSTRUCTION R6
-INDEXED_MODE R9
-REGISTER_MODE))]
-|}
-
- *)
